Test/tutorial/ImpVerifiedCompiler/ImpReductionContSem.dfy
@@ -14,56 +14,6 @@ datatype cont =
 
 type conf = (com,cont,store)
 
-datatype StepCases =
-	| SAssign(ident,aexp,cont,store)
-	| SSeq(com,com,store,cont)
-	| SIf(bexp,com,com,cont,store)
-	| SWhileDone(bexp,com,cont,store)
-	| SWhileTrue(bexp,com,cont,store)
-	| StepSkipSeq(com,cont,store)
-	| StepSkipWhile(bexp,com,cont,store)
-
-predicate stepNice(red: StepCases,conf1: conf, conf2: conf) {
-	match red {
-		case SAssign(i,a,k,s) =>
-			&& (forall id: ident :: id_in_aexp(id,a) ==> id in s)
-			&& conf1 == (CAsgn(i,a),k,s[i := aeval(s,a)])
-			&& conf2 == (CSkip,k,s)
-		case SSeq(c1,c2,s,k) =>
-			&& conf1 == (CSeq(c1, c2), k, s)
-			&& conf2 == (c1, Kseq(c2, k), s)
-		case SIf(b,c1,c2,k,s) =>
-			if (forall id: ident :: id_in_bexp(id,b) ==> id in s) then
-			&& conf1 == (CIf(b, c1, c2), k, s)
-			&& conf2 == (if beval(s, b) then c1 else c2, k, s)
-			else false
-		case SWhileDone(b,c,k,s) =>
-			&& conf1 == (CWhile(b, c), k, s)
-			&& conf2 == (CSkip, k, s)
-		case SWhileTrue(b,c,k,s) =>
-			&& conf1 == (CWhile(b, c), k, s)
-			&& conf2 == (c, Kwhile(b, c, k), s)
-		case StepSkipSeq(c,k,s) =>
-			&& conf1 == (CSkip, Kseq(c, k), s)
-			&& conf2 == (c, k, s)
-		case StepSkipWhile(b,c,k,s) =>
-			&& conf1 == (CSkip, Kwhile(b, c, k), s)
-			&& conf2 == (CWhile(b, c), k, s)
-	}
-}
-
-predicate SameCont(conf1: conf,conf2: conf) {
-	conf1.1 == conf2.1
-}
-
-predicate SameStore(conf1: conf,conf2: conf) {
-	conf1.2 == conf2.2
-}
-
-predicate SameContAndStore(conf1: conf,conf2: conf) {
-	SameCont(conf1,conf2) && SameStore(conf1,conf2)
-}
-
 predicate step(conf1: conf, conf2: conf) {
 	var (c1,k1,s1) := conf1;
 	var (c2,k2,s2) := conf2;
